Added the inlined AtomicMemWoQ;
(wip: proving the intermediate refinement)

examples/MemAtomic.v
@@ -1,7 +1,7 @@
 Require Import Bool String List.
 Require Import Lib.CommonTactics Lib.ilist Lib.Word Lib.Indexer.
 Require Import Kami.Syntax Kami.Notations Kami.Semantics Kami.Specialize Kami.Duplicate Kami.RefinementFacts.
-Require Import Kami.Wf Kami.ParametricEquiv Kami.Tactics.
+Require Import Kami.Wf Kami.ParametricSyntax Kami.ParametricEquiv Kami.Tactics.
 Require Import Ex.MemTypes Ex.SC Ex.Fifo.
 
 Set Implicit Arguments.
@@ -36,9 +36,39 @@ Section Middleman.
     with Rule "processSt" := processSt
   }.
 
+  Section MemAtomicWoQInl.
+    Variable n: nat.
+
+    Hypothesis HinName: index 0 indexSymbol (inName -- "deq") = None.
+    Hypothesis HoutName: index 0 indexSymbol (outName -- "enq") = None.
+
+    Definition memAtomicWoQInlM := META {
+      Register "mem" : Vector (Data lgDataBytes) addrSize <- Default
+
+      with Repeat Rule till n by "processLd" :=
+        Calli req <- { getReq | HinName } ();
+        Assert !#req!RqFromProc@."op";
+        Read memv <- "mem";
+        LET ldval <- #memv@[#req!RqFromProc@."addr"];
+        LET rep <- STRUCT { "data" ::= #ldval } :: Struct RsToProc;
+        Calli { setRep | HoutName } (#rep);
+        Retv
+
+      with Repeat Rule till n by "processSt" :=
+        Calli req <- { getReq | HinName } ();
+        Assert #req!RqFromProc@."op";
+        Read memv <- "mem";
+        Write "mem" <- #memv@[ #req!RqFromProc@."addr" <- #req!RqFromProc@."data" ];
+        LET rep <- STRUCT { "data" ::= $$Default } :: Struct RsToProc;
+        Calli { setRep | HoutName } (#rep);
+        Retv
+    }.
+    
+  End MemAtomicWoQInl.
+  
 End Middleman.
 
-Hint Unfold mid : ModuleDefs.
+Hint Unfold mid memAtomicWoQInlM : ModuleDefs.
 Hint Unfold RqFromProc RsToProc getReq setRep exec processLd processSt : MethDefs.
 
 Section MemAtomic.
@@ -61,11 +91,15 @@ Section MemAtomic.
   Definition ioms (i: nat) := duplicate iom i.
 
   Definition memAtomicWoQ := ConcatMod (mids n) minst.
+  Definition memAtomicWoQInl :=
+    modFromMeta (memAtomicWoQInlM "rqFromProc" "rsToProc" addrSize lgDataBytes n
+                                  eq_refl eq_refl).
   Definition memAtomic := ConcatMod (ioms n) minst.
 
 End MemAtomic.
 
-Hint Unfold minst inQ outQ ioQ midQ mids iom ioms memAtomicWoQ memAtomic : ModuleDefs.
+Hint Unfold minst inQ outQ ioQ midQ mids iom ioms
+     memAtomicWoQInl memAtomicWoQ memAtomic : ModuleDefs.
 
 Section Facts.
   Variables (addrSize fifoSize lgDataBytes: nat).
@@ -100,6 +134,12 @@ Section Facts.
   Qed.
   Hint Resolve ioms_ModEquiv.
 
+  Lemma memAtomicWoQInl_ModEquiv:
+    ModPhoasWf (memAtomicWoQInl addrSize lgDataBytes n).
+  Proof.
+    kequiv.
+  Qed.
+
   Lemma memAtomicWoQ_ModEquiv:
     ModPhoasWf (memAtomicWoQ addrSize lgDataBytes n).
   Proof.
@@ -115,7 +155,8 @@ Section Facts.
 End Facts.
 
 Hint Immediate midQ_ModEquiv iom_ModEquiv
-     mids_ModEquiv ioms_ModEquiv memAtomicWoQ_ModEquiv memAtomic_ModEquiv.
+     mids_ModEquiv ioms_ModEquiv
+     memAtomicWoQ_ModEquiv memAtomicWoQInl_ModEquiv memAtomic_ModEquiv.
 
 Section MemAtomicWoQ.
   Variables (addrSize fifoSize lgDataBytes: nat).
@@ -135,3 +176,36 @@ Section MemAtomicWoQ.
 
 End MemAtomicWoQ.
 
+Require Import Lib.FMap Lib.Reflection.
+
+Section MemAtomicWoQInl.
+  Variables addrSize lgDataBytes: nat.
+  Variable n: nat.
+
+  Definition memAtomicWoQ_regMap (r: RegsT) := r.
+  Definition memAtomicWoQ_ruleMap (o: RegsT) (rn: string) := Some rn.
+
+  Lemma memAtomicWoQInl_refines_memAtomicWoQ:
+    memAtomicWoQInl addrSize lgDataBytes n <<== memAtomicWoQ addrSize lgDataBytes n.
+  Proof.
+    apply stepRefinement with (ruleMap:= memAtomicWoQ_ruleMap) (theta:= memAtomicWoQ_regMap);
+      [admit|].
+
+    intros; clear H.
+    apply SemFacts.step_zero in H0; [|reflexivity]; dest.
+    destruct l as [ann ds cs]; simpl in *; subst; cbn.
+    destruct ann as [r|].
+
+    - inv H0.
+      + exists (M.empty _); cbn; split; auto.
+        admit. (* empty-step *)
+
+      + unfold memAtomicWoQ_ruleMap.
+        admit.
+
+    - inv H0; exists (M.empty _); cbn; split; auto.
+      admit. (* empty-step *)
+  Admitted.
+
+End MemAtomicWoQInl.
+  
